More memory safety for Curve25519

crypto_hst/ec/Hacl.EC.Curve25519.Point.fst
@@ -53,7 +53,7 @@ type distinct (a:point) (b:point) =
 
 let op_Plus_Plus_Plus = TSet.union
 
-let refs p = TSet.singleton (Buff (get_x p)) +++ TSet.singleton (Buff (get_y p)) +++ TSet.singleton (Buff (get_z p))
+let refs p : GTot (TSet.set Heap.aref) = arefs (only (get_x p) ++ only (get_y p) ++ (only (get_z p)))
 
 val make: bigint -> bigint -> bigint -> Tot point
 let make x y z = Point x y z
@@ -68,7 +68,6 @@ val swap_conditional_aux': a:bigint -> b:bigint{disjoint a b} ->
       (* (\* /\ EqSub h0 a 0 h1 a 0 ctr /\ EqSub h0 b 0 h1 b 0 ctr *\) *)
       (* /\ partialSwap h0 h1 is_swap (w ctr) a b)) *)
 let rec swap_conditional_aux' a b swap ctr =
-  (* admit(); // TODO *)
   (* let h0 = HST.get() in *)
   if U32 (nlength =^ ctr) then ()
   else begin
@@ -119,17 +118,80 @@ let rec swap_conditional_aux a b swap =
   (* let h1 = HST.get() in  *)
   (* swap_conditional_aux_lemma h0 h1 a b swap   *)
 
-#reset-options "--lax"
+#reset-options "--initial_fuel 0 --max_fuel 0 --z3timeout 5"
 
-(* TODO: lift from the modifies_2 to the modifies_bufs_and_refs *)
+(* For simplicity, assuming that the point coordinates have been allocated on the same frame.
+   Ideally in the same buffer *)
+type same_frame (p:point) =
+  frameOf (get_x p) = frameOf (get_y p) /\ frameOf (get_x p) = frameOf (get_z p)
+type same_frame_2 (p:point) (p':point) =
+  same_frame p /\ same_frame p' /\ frameOf (get_x p) = frameOf (get_x p')
+
+let frame_of (p:point{same_frame p}) : GTot HH.rid = frameOf (get_x p)
+
+val helper_lemma: #t:Type -> a:buffer t -> b:buffer t -> Lemma
+  (requires (True))
+  (ensures  (arefs (only a ++ only b) == !{as_ref a, as_ref b}))
+let helper_lemma #t a b =
+  let s =  only a ++ only b in
+  let s' = !{as_ref a, as_ref b} in
+  assert(TSet.mem (Buff a) s);
+  assert(TSet.mem (Buff b) s);
+  TSet.lemma_equal_intro (arefs s) s'
+
+let helper_lemma_2 r h0 h1 (sub:TSet.set Heap.aref) (s:TSet.set Heap.aref) : Lemma
+  (requires (TSet.subset sub s /\ modifies_ref r sub h0 h1))
+  (ensures  (modifies_ref r s h0 h1))
+  = ()
+
+let helper_lemma_3 r h0 h1 h2 s : Lemma
+  (requires (HS.modifies_ref r s h0 h1 /\ HS.modifies_ref r s h1 h2))
+  (ensures  (HS.modifies_ref r s h0 h2))
+  = ()
+
+let prop_1 h0 h1 (a:point) (b:point) : GTot Type0 =
+  same_frame_2 a b
+  /\ (forall (#t:Type) (b':buffer t). (frameOf b' = frame_of a /\ B.live h0 b'
+       /\ disjoint_from_bufs b' (only (get_x a) ++ only (get_y a) ++ only (get_z a)
+				    ++ only (get_x b) ++ only (get_y b) ++ only (get_z b) ))
+				    ==> equal h0 b' h1 b')
+
+#reset-options "--initial_fuel 0 --max_fuel 0 --z3timeout 20"
+
+let helper_lemma_4 r h0 h1 h2 h3 a b : Lemma
+  (requires ( (forall (#t:Type) (b':buffer t). (frameOf b' = frame_of a /\ B.live h0 b'
+      /\ disjoint b' (get_x a) /\ disjoint b' (get_x b))  ==> equal h0 b' h1 b')
+    /\ (forall (#t:Type) (b':buffer t). (frameOf b' = frame_of a /\ B.live h1 b'
+      /\ disjoint b' (get_y a) /\ disjoint b' (get_y b))  ==> equal h1 b' h2 b')
+    /\ (forall (#t:Type) (b':buffer t). (frameOf b' = frame_of a /\ B.live h2 b'
+      /\ disjoint b' (get_z a) /\ disjoint b' (get_z b))  ==> equal h2 b' h3 b')
+     /\ same_frame_2 a b ))
+   (ensures  (prop_1 h0 h3 a b))
+  = let s = only (get_x a) ++ only (get_y a) ++ only (get_z a)
+	    ++ only (get_x b) ++ only (get_y b) ++ only (get_z b) in
+    assert(TSet.mem (Buff (get_x a)) s);
+    assert(TSet.mem (Buff (get_y a)) s);
+    assert(TSet.mem (Buff (get_z a)) s);
+    assert(TSet.mem (Buff (get_x b)) s);
+    assert(TSet.mem (Buff (get_y b)) s);
+    assert(TSet.mem (Buff (get_z b)) s);
+    assert(forall (#t:Type) (b':buffer t). disjoint_from_bufs b' s
+	     ==> (disjoint b' (get_x a) /\ disjoint b' (get_x b)));
+    assert(forall (#t:Type) (b':buffer t). disjoint_from_bufs b' s
+	     ==> (disjoint b' (get_y a) /\ disjoint b' (get_y b)));
+    assert(forall (#t:Type) (b':buffer t). disjoint_from_bufs b' s
+	     ==> (disjoint b' (get_z a) /\ disjoint b' (get_z b)))
+
 val swap_conditional:
-  a:point -> b:point{distinct a b} ->
+  a:point{same_frame a} -> b:point{distinct a b /\ same_frame b} ->
   is_swap:s64{v is_swap = pow2 platform_size -1 \/ v is_swap = 0} ->
   STStack unit
-    (requires (fun h -> live h a /\ live h b))
+    (requires (fun h -> live h a /\ live h b /\ same_frame_2 a b))
       (* onCurve h a /\ onCurve h b)) *)
     (ensures (fun h0 _ h1 -> live h1 a /\ live h1 b
-      /\ modifies_bufs_and_refs (refs a +++ refs b) TSet.empty h0 h1))
+      /\ HS.modifies_one (frame_of a) h0 h1
+      /\ HS.modifies_ref (frame_of a) (refs a ++ refs b) h0 h1
+      /\ prop_1 h0 h1 a b))
       (* (onCurve h0 a /\ onCurve h0 b) /\ (onCurve h1 a /\ onCurve h1 b) *)
       (* (\* /\ modifies (refs a +++ refs b) h0 h1  *\) *)
       (* /\ (v is_swap = 0 ==>  *)
@@ -137,44 +199,106 @@ val swap_conditional:
       (* /\ (v is_swap = pow2 platform_size - 1 ==>  *)
       (* 	  ((pointOf h1 a) == (pointOf h0 b) /\ (pointOf h1 b) == (pointOf h0 a))) )) *)
 let swap_conditional a b is_swap =
-  (* let h0 = HST.get() in *)
+  let h0 = HST.get() in
   swap_conditional_aux (get_x a) (get_x b) is_swap;
-  (* let h1 = HST.get() in *)
+  let h1 = HST.get() in
+  lemma_reveal_modifies_2 (get_x a) (get_x b) h0 h1;
+  (* assert(disjoint (get_x a) (get_y a)); assert(disjoint (get_x b) (get_y a)); *)
+  (* no_upd_lemma_2 h0 h1 (get_x a) (get_x b) (get_y a); *)
+  cut (live h1 a /\ live h1 b);
   (* norm_lemma h0 h1 (get_y a) !{getRef (get_x a), getRef (get_x b)}; *)
   (* norm_lemma h0 h1 (get_y b) !{getRef (get_x a), getRef (get_x b)}; *)
   swap_conditional_aux (get_y a) (get_y b) is_swap;
-  (* let h2 = HST.get() in *)
+  let h2 = HST.get() in
+  cut (live h2 a /\ live h2 b);
+  lemma_reveal_modifies_2 (get_y a) (get_y b) h1 h2;
   (* let mods = (hide !{getRef (get_x a), getRef (get_x b), getRef (get_y a), getRef (get_y b)}) in *)
   (* cut(modifies (reveal mods) h0 h2);  *)
   (* cut(not(FStar.Set.mem (Ref (getRef (get_z b))) (reveal mods)) /\ not(FStar.Set.mem (Ref (getRef (get_z a))) (reveal mods)));  *)
   (* enorm_lemma h0 h2 (get_z a) mods; *)
   (* enorm_lemma h0 h2 (get_z b) mods; *)
-  swap_conditional_aux (get_z a) (get_z b) is_swap(* ; *)
-  (* let h3 = HST.get() in *)
-  (* swap_conditional_lemma h0 h1 h2 h3 a b is_swap *)
+  swap_conditional_aux (get_z a) (get_z b) is_swap;
+  let h3 = HST.get() in
+  cut (live h3 a /\ live h3 b);
+  lemma_reveal_modifies_2 (get_z a) (get_z b) h2 h3;
+  assert(HS.modifies_one (frame_of a) h0 h3);
+  helper_lemma (get_x a) (get_x b);
+  helper_lemma (get_y a) (get_y b);
+  helper_lemma (get_z a) (get_z b);
+  let s = (refs a ++ refs b) in
+  helper_lemma_2 (frame_of a) h0 h1 (arefs (only (get_x a) ++ only (get_x b))) s;
+  helper_lemma_2 (frame_of a) h1 h2 (arefs (only (get_y a) ++ only (get_y b))) s;
+  helper_lemma_2 (frame_of a) h2 h3 (arefs (only (get_z a) ++ only (get_z b))) s;
+  helper_lemma_3 (frame_of a) h0 h1 h2 s;
+  helper_lemma_3 (frame_of a) h0 h2 h3 s;
+  helper_lemma_4 (frame_of a) h0 h1 h2 h3 a b;
+  assert(HS.modifies_ref (frame_of a) s h0 h3);
+  ()
+
+val helper_lemma': #t:Type -> a:buffer t -> Lemma
+  (requires (True))
+  (ensures  (arefs (only a) == !{as_ref a}))
+let helper_lemma' #t a =
+  let s =  only a in
+  let s' = !{as_ref a} in
+  assert(TSet.mem (Buff a) s);
+  TSet.lemma_equal_intro (arefs s) s'
+
+let prop_2 h0 h1 (a:point) : GTot Type0 =
+  same_frame a
+  /\ (forall (#t:Type) (b':buffer t). (frameOf b' = frame_of a /\ B.live h0 b'
+       /\ disjoint_from_bufs b' (only (get_x a) ++ only (get_y a) ++ only (get_z a)))
+				    ==> equal h0 b' h1 b')
+
+let helper_lemma_4' r h0 h1 h2 h3 a : Lemma
+  (requires ( (forall (#t:Type) (b':buffer t). (frameOf b' = frame_of a /\ B.live h0 b'
+      /\ disjoint b' (get_x a))  ==> equal h0 b' h1 b')
+    /\ (forall (#t:Type) (b':buffer t). (frameOf b' = frame_of a /\ B.live h1 b'
+      /\ disjoint b' (get_y a))  ==> equal h1 b' h2 b')
+    /\ (forall (#t:Type) (b':buffer t). (frameOf b' = frame_of a /\ B.live h2 b'
+      /\ disjoint b' (get_z a))  ==> equal h2 b' h3 b')
+     /\ same_frame a ))
+   (ensures  (prop_2 h0 h3 a))
+  = let s = only (get_x a) ++ only (get_y a) ++ only (get_z a) in
+    assert(TSet.mem (Buff (get_x a)) s);
+    assert(TSet.mem (Buff (get_y a)) s);
+    assert(TSet.mem (Buff (get_z a)) s);
+    assert(forall (#t:Type) (b':buffer t). disjoint_from_bufs b' s
+	     ==> (disjoint b' (get_x a)));
+    assert(forall (#t:Type) (b':buffer t). disjoint_from_bufs b' s
+	     ==> (disjoint b' (get_y a)));
+    assert(forall (#t:Type) (b':buffer t). disjoint_from_bufs b' s
+	     ==> (disjoint b' (get_z a)))
+
+#reset-options "--initial_fuel 0 --max_fuel 0 --z3timeout 100"
 
 val copy:
-  a:point -> b:point{distinct a b} ->
+  a:point{same_frame a} -> b:point{distinct a b} ->
   STStack unit
     (requires (fun h -> live h a /\ live h b))
       (* /\ onCurve h b)) *)
-    (ensures (fun h0 _ h1 -> live h1 a /\ modifies_bufs_and_refs (refs a) TSet.empty h0 h1
+    (ensures (fun h0 _ h1 -> live h1 a /\ live h1 b
+      /\ HS.modifies_one (frame_of a) h0 h1
+      /\ HS.modifies_ref (frame_of a) (refs a) h0 h1
+      /\ prop_2 h0 h1 a))
       (* (live h0 a) /\ (onCurve h1 a) /\ (onCurve h0 b) /\ (onCurve h1 b) *)
       (* /\ (pointOf h1 a = pointOf h0 b) /\ (pointOf h1 b = pointOf h0 b) *)
       (* /\ (modifies (refs a) h0 h1) *)
-      ))
 let copy a b =
-  (* admit(); // TODO *)
-  (* let h0 = HST.get() in *)
+  let h0 = HST.get() in
   blit (get_x b) 0ul (get_x a) 0ul nlength;
-  (* let h1 = HST.get() in  *)
+  let h1 = HST.get() in
+  cut (live h1 a /\ live h1 b);
+  lemma_reveal_modifies_1 (get_x a) h0 h1;
   (* norm_lemma h0 h1 (get_x b) (!{getRef (get_x a)});  *)
   (* norm_lemma h0 h1 (get_y b) (!{getRef (get_x a)});  *)
   (* norm_lemma h0 h1 (get_z b) (!{getRef (get_x a)});  *)
   (* bignum_live_lemma h0 h1 (get_y a) (!{getRef (get_x a)});  *)
   (* bignum_live_lemma h0 h1 (get_z a) (!{getRef (get_x a)});  *)
   blit (get_y b) 0ul (get_y a) 0ul nlength;
-  (* let h2 = HST.get() in *)
+  let h2 = HST.get() in
+  cut (live h2 a /\ live h2 b);
+  lemma_reveal_modifies_1 (get_y a) h1 h2;
   (* norm_lemma h1 h2 (get_x b) (!{getRef (get_y a)});  *)
   (* norm_lemma h1 h2 (get_y b) (!{getRef (get_y a)}); *)
   (* norm_lemma h1 h2 (get_z b) (!{getRef (get_y a)});  *)
@@ -182,7 +306,9 @@ let copy a b =
   (* norm_lemma h1 h2 (get_x a) (!{getRef (get_y a)});  *)
   (* bignum_live_lemma h1 h2 (get_z a) (!{getRef (get_y a)}); *)
   blit (get_z b) 0ul (get_z a) 0ul nlength;
-  (* let h3 = HST.get() in *)
+  let h3 = HST.get() in
+  cut (live h2 a /\ live h2 b);
+  lemma_reveal_modifies_1 (get_z a) h2 h3;
   (* norm_lemma h2 h3 (get_x b) (!{getRef (get_z a)}); *)
   (* norm_lemma h2 h3 (get_y b) (!{getRef (get_z a)}); *)
   (* norm_lemma h2 h3 (get_z b) (!{getRef (get_z a)}); *)
@@ -190,63 +316,102 @@ let copy a b =
   (* norm_lemma_2 h1 h2 (get_y b) (get_y a);  *)
   (* norm_lemma h2 h3 (get_y a) (!{getRef (get_z a)});  *)
   (* norm_lemma_2 h2 h3 (get_z b) (get_z a) *)
+  helper_lemma' (get_x a);
+  helper_lemma' (get_y a);
+  helper_lemma' (get_z a);
+  let s = (refs a) in
+  helper_lemma_2 (frame_of a) h0 h1 (arefs (only (get_x a))) s;
+  helper_lemma_2 (frame_of a) h1 h2 (arefs (only (get_y a))) s;
+  helper_lemma_2 (frame_of a) h2 h3 (arefs (only (get_z a))) s;
+  helper_lemma_3 (frame_of a) h0 h1 h2 s;
+  helper_lemma_3 (frame_of a) h0 h2 h3 s;
+  helper_lemma_4' (frame_of a) h0 h1 h2 h3 a;
+  assert(HS.modifies_ref (frame_of a) s h0 h3);
   ()
 
 #reset-options "--initial_fuel 0 --max_fuel 0"
 
 val swap:
-  a:point -> b:point{distinct a b} ->
+  a:point -> b:point{distinct a b /\ same_frame b} ->
   STStack unit
     (requires (fun h -> live h a /\ live h b))
       (* onCurve h a /\ live h b)) *)
-    (ensures (fun h0 _ h1 -> live h1 b /\ modifies_bufs_and_refs (refs b) TSet.empty h0 h1
+    (ensures (fun h0 _ h1 -> live h1 b /\ live h1 a
+      /\ HS.modifies_one (frame_of b) h0 h1
+      /\ HS.modifies_ref (frame_of b) (refs b) h0 h1
+      /\ prop_2 h0 h1 b ))
       (* onCurve h0 a /\ live h0 b /\ onCurve h1 b /\ live h1 a *)
       (* /\ (pointOf h0 a) == (pointOf h1 b) *)
       (* (\* /\ modifies (FStar.Set.union (refs a) (refs b)) h0 h1)) *\) *)
-      ))
 let swap a b =
   copy b a
 
-(* TODO *)
-#reset-options "--lax"
+val helper_lemma_5: h0:mem -> h1:mem -> a:point -> b:point -> Lemma
+  (requires (prop_2 h0 h1 a /\ distinct a b /\ live h0 b /\ same_frame_2 a b))
+  (ensures  (live h1 b))
+let helper_lemma_5 h0 h1 a b =
+  let x = get_x b in
+  let y = get_y b in
+  let z = get_z b in
+  let s = (only (get_x a) ++ only (get_y a) ++ only (get_z a)) in
+  assert(disjoint_from_bufs x s);
+  assert(disjoint_from_bufs y s);
+  assert(disjoint_from_bufs z s)
+
+#reset-options "--initial_fuel 0 --max_fuel 0 --z3timeout 100"
 
 val swap_both:
-  a:point -> b:point{distinct a b} -> c:point{distinct c a /\ distinct c b} ->
-  d:point{distinct d a /\ distinct d b /\ distinct d c} ->
-  STStack unit
+  a:point -> b:point{distinct a b /\ same_frame_2 a b} ->
+  c:point{distinct c a /\ distinct c b /\ same_frame_2 b c} ->
+  d:point{distinct d a /\ distinct d b /\ distinct d c /\ same_frame_2 c d} -> STStack unit
     (requires (fun h -> live h a /\ live h b /\ live h c /\ live h d))
       (* onCurve h a /\ onCurve h b /\ live h c /\ live h d)) *)
     (ensures (fun h0 _ h1 -> live h1 a /\ live h1 b /\ live h1 c /\ live h1 d
-      /\ modifies_bufs_and_refs ((refs a) +++ (refs b) +++ (refs c) +++ (refs d)) TSet.empty h0 h1
+      /\ HS.modifies_one (frame_of a) h0 h1
+      /\ HS.modifies_ref (frame_of a) (refs a ++ refs b ++ refs c ++ refs d) h0 h1 ))
       (* onCurve h0 a /\ onCurve h0 b /\ live h0 c /\ live h0 d *)
       (* /\ onCurve h1 c /\ onCurve h1 d /\ live h1 a /\ live h1 b *)
       (* /\ (pointOf h0 a) == (pointOf h1 c) /\ (pointOf h0 b) == (pointOf h1 d) *)
-    ))
 let swap_both a b c d =
   (* admit(); // OK *)
-  (* let h0 = HST.get() in *)
+  let h0 = HST.get() in
   copy c a;
-  (* let h1 = HST.get() in *)
+  let h1 = HST.get() in
+  helper_lemma_5 h0 h1 c a;
+  helper_lemma_5 h0 h1 c b;
+  helper_lemma_5 h0 h1 c d;
   (* let set01 = erefs c in  *)
   (* distinct_lemma c b;  *)
   (* distinct_lemma c d;  *)
   (* on_curve_lemma h0 h1 b set01;  *)
   (* live_lemma h0 h1 d set01;  *)
   copy d b;
-  (* let h2 = HST.get() in *)
+  let h2 = HST.get() in
+  helper_lemma_5 h1 h2 d a;
+  helper_lemma_5 h1 h2 d b;
+  helper_lemma_5 h1 h2 d c;
   (* distinct_lemma d c;  *)
   (* distinct_lemma d a; *)
   (* distinct_lemma d b; *)
   (* on_curve_lemma h1 h2 c (erefs d); *)
   (* live_lemma h1 h2 a (erefs d); *)
   (* live_lemma h1 h2 b (erefs d) *)
+  let s = (refs a ++ refs b ++ refs c ++ refs d) in
+  helper_lemma_2 (frame_of a) h0 h1 (refs c) s;
+  helper_lemma_2 (frame_of a) h1 h2 (refs d) s;
+  helper_lemma_3 (frame_of a) h0 h1 h2 s;
   ()
 
-val copy2: p':point -> q':point{distinct p' q'} -> p:point{distinct p p' /\ distinct p q'} ->
-  q:point{distinct q p' /\ distinct q q'} -> STStack unit
+#reset-options "--initial_fuel 0 --max_fuel 0 --z3timeout 100"
+
+val copy2: p':point -> q':point{distinct p' q' /\ same_frame_2 p' q'} ->
+  p:point{distinct p p' /\ distinct p q' /\ same_frame_2 p q'} ->
+  q:point{distinct q p' /\ distinct q q' /\ same_frame_2 p q} -> STStack unit
     (requires (fun h -> live h p' /\ live h q' /\ live h p /\ live h q))
       (* live h p' /\ live h q' /\ onCurve h p /\ onCurve h q )) *)
-    (ensures (fun h0 _ h1 -> live h1 p' /\ live h1 q' /\ modifies_bufs_and_refs (refs p' +++ refs q') TSet.empty h0 h1))
+    (ensures (fun h0 _ h1 -> live h1 p' /\ live h1 q' /\ live h1 p /\ live h1 q
+      /\ HS.modifies_one (frame_of p) h0 h1
+      /\ HS.modifies_ref (frame_of p) (refs p' +++ refs q') h0 h1 ))
       (* onCurve h1 p' /\ onCurve h1 q' /\ onCurve h1 p /\ onCurve h1 q  *)
       (* /\ onCurve h0 p /\ onCurve h0 q *)
       (* (\* /\ (modifies (FStar.Set.union (refs p') (refs q')) h0 h1) *\) *)
@@ -254,22 +419,32 @@ val copy2: p':point -> q':point{distinct p' q'} -> p:point{distinct p p' /\ dist
       (* /\ (pointOf h1 q' == pointOf h0 q) )) *)
 let copy2 p' q' p q =
   (* admit(); // OK *)
-  (* let h0 = HST.get() in *)
+  let h0 = HST.get() in
   copy p' p;
-  (* let h1 = HST.get() in *)
+  let h1 = HST.get() in
+  helper_lemma_5 h0 h1 p' q';
+  helper_lemma_5 h0 h1 p' p;
+  helper_lemma_5 h0 h1 p' q;
   (* let set01 = (erefs p') in  *)
   (* distinct_lemma p' q;  *)
   (* distinct_lemma p' q';  *)
   (* on_curve_lemma h0 h1 q set01;  *)
   (* live_lemma h0 h1 q' set01;   *)
   copy q' q;
-  (* let h2 = HST.get() in *)
+  let h2 = HST.get() in
+  helper_lemma_5 h1 h2 q' p';
+  helper_lemma_5 h1 h2 q' p;
+  helper_lemma_5 h1 h2 q' q;
   (* distinct_lemma q' p';  *)
   (* distinct_lemma q' p; *)
   (* distinct_lemma q' q;  *)
   (* on_curve_lemma h1 h2 p' (erefs q');  *)
   (* on_curve_lemma h1 h2 p (erefs q');  *)
   (* on_curve_lemma h1 h2 q (erefs q') *)
+  let s = (refs p' ++ refs q') in
+  helper_lemma_2 (frame_of p) h0 h1 (refs p') s;
+  helper_lemma_2 (frame_of p) h1 h2 (refs q') s;
+  helper_lemma_3 (frame_of p) h0 h1 h2 s;
   ()
 
 #reset-options "--initial_fuel 0 --max_fuel 0"
